\documentclass{report}

\begin{document}

\begin{equation}
R \bowtie_\theta S=\{r \cup s:r \in R,s \in S,f_\theta(t \cup s)\}
\end{equation}
\begin{equation}
\sigma_\phi(_{\sigma_{\phi_1}(R) \times \sigma_{\phi_2}(S)})=\{r \cup s:r \in R,s \in S,f_\phi(t,s) \cap f_{\phi_1}(r) \cap f_{\phi_2}(s)\}
\end{equation}
\begin{equation}
f_\theta(t \cup s)=f_{\theta_1}(t,s) \cap f_{\theta_2}(t) \cap f_{\theta_3}(s)
\end{equation}
\begin{equation}
\left.
\begin{array}{lll}
f_{\theta_1}(t,s)=f_\phi(t,s)\\
f_{\theta_2}(t)=f_{\phi_1}(t)\\
f_{\theta_3}(s)=f_{\phi_2}(s)
\end{array} 
\right\}
\Rightarrow
R \bowtie_\theta S=\sigma_\phi(\sigma_{\phi_1}(R) \times \sigma_{\phi_2}(S))
\end{equation}

\end{document}